\documentclass{article}
\usepackage{amssymb}
\usepackage{amsmath}
\usepackage{centernot}
\DeclareMathOperator*{\Union}{\bigcup}

\begin{document}

\title{EE351k: Homework 4}
\author{Anthony Weems}
\date{\today}
\maketitle

% Problem 1
\subsection{}

\begin{align*}
    \mathbb{P}(S_{dot}|R_{dot}) &= \dfrac{\mathbb{P}(R_{dot}|S_{dot}) * \mathbb{P}(S_{dot})}{\mathbb{P}(R_{dot}|S_{dot}) * \mathbb{P}(S_{dot}) + \mathbb{P}(R_{dot}|S_{dash}) * \mathbb{P}(S_{dash})} \\
    &=\dfrac{\frac{5}{6} * \frac{2}{3}}{\frac{5}{6} * \frac{2}{3} + \frac{1}{5} * \frac{1}{3}} =\dfrac{25}{28}
\end{align*}

% Problem 2
\subsection{}

\begin{enumerate}
    \item[a.] Second ball is magenta: \\
        Event $M_r$ = $r^{th}$ urn, second ball magenta
        \begin{align*}
            \mathbb{P}(M_r) &= \dfrac{\binom{r-1}{1}}{\binom{n-1}{1}} * \dfrac{\binom{n-r}{1}}{\binom{n-2}{1}} + \dfrac{\binom{n-r}{1}}{\binom{n-1}{1}} * \dfrac{\binom{n-r-1}{1}}{\binom{n-2}{1}} \\
            &= \dfrac{(r-1)(n-r) + (n-r)(n-r-1)}{(n-1)(n-2)} \\
            &= \dfrac{(n-r)((r-1)+(n-r-1))}{(n-1)(n-2)} \\
            &= \dfrac{(n-r)}{(n-1)}
        \end{align*}
        Event A = random urn, second ball magenta
        \begin{align*}
            \mathbb{P}(A) &= \frac{1}{n}\sum\limits_{r=1}^{n}\mathbb{P}(M_r) \\
            &= \frac{1}{n}\sum\limits_{r=1}^{n}\frac{(n-r)}{(n-1)} \\
            &= \frac{1}{n} * \frac{n}{2} \\
            &= \frac{1}{2}
        \end{align*}
    \item[b.] Second ball is magenta given first is magenta: \\
        Event $M_r$ = $r^{th}$ urn, second ball magenta
        \begin{align*}
            \mathbb{P}(M_r) &= \dfrac{(n-r)}{(n-1)}
        \end{align*}
        Event $Q_r$ = $r^{th}$ urn, first ball magenta
        \begin{align*}
            \mathbb{P}(Q_r) &= \dfrac{\binom{n-r}{1}}{\binom{n-1}{1}} \\
            &= \dfrac{(n-r)}{(n-1)}
        \end{align*}
        Event $R_r$ = $r^{th}$ urn, second ball magenta given first ball magenta
        \begin{align*}
            \mathbb{P}(A) &= \mathbb{P}(M_r|Q_r) = \dfrac{\mathbb{P}(M_r \cap Q_r)}{\mathbb{P}(Q_r)} \\
            &= \dfrac{\dfrac{n-r}{n-1} * \dfrac{n-r-1}{n-2}}{\frac{n-r}{n-1}} \\
            &= \dfrac{n-r-1}{n-2}
        \end{align*}
        Event A = random urn, second ball magenta given first ball magenta
        \begin{align*}
            \mathbb{P}(A) &= \frac{1}{n}\sum\limits_{r=1}^{n}\mathbb{P}(R_r) \\
            &= \sum\limits_{r=1}^{n}\frac{n-r-1}{n^2-2n} \\
            &= \dfrac{n-3}{2(n-2)}
        \end{align*}
\end{enumerate}

% Problem 3
\subsection{}
$\mathbb{P}(X=0) = \dfrac{\binom{5}{0}\binom{20}{4}}{\binom{25}{4}} = 0.3830$ \\
$\mathbb{P}(X=1) = \dfrac{\binom{5}{1}\binom{20}{3}}{\binom{25}{4}} = 0.4506$ \\
$\mathbb{P}(X=2) = \dfrac{\binom{5}{2}\binom{20}{2}}{\binom{25}{4}} = 0.1502$ \\
$\mathbb{P}(X=3) = \dfrac{\binom{5}{3}\binom{20}{1}}{\binom{25}{4}} = 0.0158$ \\
$\mathbb{P}(X=4) = \dfrac{\binom{5}{4}\binom{20}{0}}{\binom{25}{4}} = 0.0004$

% Problem 4
\subsection{}

\begin{enumerate}
	\item[a.] $\mathbb{P}(D) = \mathbb{P}(D \cap B_1) + \mathbb{P}(D \cap B_2) + \mathbb{P}(D \cap B_3)
	                         = \frac{1}{3} * (\frac{1}{8} + \frac{3}{8} + \frac{2}{8}) = \frac{1}{4}$
	\item[b.] $\mathbb{P}(B_2 | D) = \dfrac{\mathbb{P}(B_2) * \mathbb{P}(D | B_2)}{\mathbb{P}(D)}
                                   = \dfrac{\frac{1}{3} * \frac{3}{8}}{\frac{1}{4}} = \frac{1}{2}$
\end{enumerate}

% Problem 5
\subsection{}
$q := 1 - p$
\begin{enumerate}
	\item[a.] $\mathbb{P}(A) = \sum\limits_{n=0}^{\infty}p * q^{3n} 
                               = p * \sum\limits_{n=0}^{\infty}{q^3}^n 
                               = \dfrac{p}{1 - q^3}$
	\item[b.] $\mathbb{P}(B) = \sum\limits_{n=0}^{\infty}p * q^{3n + 1}
                               = p * q * \sum\limits_{n=0}^{\infty}{q^3}^n
                               = \dfrac{p * q}{1 - q^3}$
\end{enumerate}

% Problem 6
\subsection{}
$X_{r_1}$ is the number of balls in $r_1$ boxes \\
$p_{X_{r_1}}(k) = \binom{n}{k}(\frac{r_1}{n})^{k}(1 - \frac{r_1}{n})^{n-k} $

\end{document}
