\documentclass{article}
\usepackage{amssymb}
\usepackage{amsmath}
\usepackage{centernot}
\DeclareMathOperator*{\Union}{\bigcup}

\begin{document}

\title{EE351k: Homework 2}
\author{Anthony Weems}
\date{\today}
\maketitle

% Problem 1
\subsection{}

\begin{align*}
    \mathbb{P}(S_{dot}|R_{dot}) &= \dfrac{\mathbb{P}(R_{dot}|S_{dot}) * \mathbb{P}(S_{dot})}{\mathbb{P}(R_{dot}|S_{dot}) * \mathbb{P}(S_{dot}) + \mathbb{P}(R_{dot}|S_{dash}) * \mathbb{P}(S_{dash})} \\
    &=\dfrac{\frac{5}{6} * \frac{2}{3}}{\frac{5}{6} * \frac{2}{3} + \frac{1}{5} * \frac{1}{3}} \\
    &=\dfrac{25}{28}
\end{align*}

% Problem 2
\subsection{}

\begin{enumerate}
    \item[a.] Second ball is magenta: \\
        Event \(M_r\) = \(r^{th}\) urn, second ball magenta
        \begin{align*}
            \mathbb{P}(M_r) &= \dfrac{\binom{r-1}{1}}{\binom{n-1}{1}} * \dfrac{\binom{n-r}{1}}{\binom{n-2}{1}} + \dfrac{\binom{n-r}{1}}{\binom{n-1}{1}} * \dfrac{\binom{n-r-1}{1}}{\binom{n-2}{1}} \\
            &= \dfrac{(r-1)(n-r) + (n-r)(n-r-1)}{(n-1)(n-2)} \\
            &= \dfrac{(n-r)((r-1)+(n-r-1))}{(n-1)(n-2)} \\
            &= \dfrac{(n-r)}{(n-1)}
        \end{align*}
        Event A = random urn, second ball magenta
        \begin{align*}
            \mathbb{P}(A) &= \frac{1}{n}\sum\limits_{r=1}^{n}\mathbb{P}(M_r) \\
            &= \frac{1}{n}\sum\limits_{r=1}^{n}\frac{(n-r)}{(n-1)} \\
            &= \frac{1}{n} * \frac{n}{2} \\
            &= \frac{1}{2}
        \end{align*}
    \item[b.] Second ball is magenta given first is magenta: \\
        Event \(M_r\) = \(r^{th}\) urn, second ball magenta
        \begin{align*}
            \mathbb{P}(M_r) &= \dfrac{(n-r)}{(n-1)}
        \end{align*}
        Event \(Q_r\) = \(r^{th}\) urn, first ball magenta
        \begin{align*}
            \mathbb{P}(Q_r) &= \dfrac{\binom{n-r}{1}}{\binom{n-1}{1}} \\
            &= \dfrac{(n-r)}{(n-1)}
        \end{align*}
        Event \(R_r\) = \(r^{th}\) urn, second ball magenta given first ball magenta
        \begin{align*}
            \mathbb{P}(A) &= \mathbb{P}(M_r|Q_r) = \dfrac{\mathbb{P}(M_r \cap Q_r)}{\mathbb{P}(Q_r)} \\
            &= \dfrac{\dfrac{n-r}{n-1} * \dfrac{n-r-1}{n-2}}{\frac{n-r}{n-1}} \\
            &= \dfrac{n-r-1}{n-2} \\
        \end{align*}
        Event A = random urn, second ball magenta given first ball magenta
        \begin{align*}
            \mathbb{P}(A) &= \frac{1}{n}\sum\limits_{r=1}^{n}\mathbb{P}(R_r) \\
            &= \sum\limits_{r=1}^{n}\frac{n-r-1}{n^2-2n} \\
            &= \dfrac{n-3}{2(n-2)}
        \end{align*}
\end{enumerate}

% Problem 3
\subsection{}

% Problem 4
\subsection{}

% Problem 5
\subsection{}

% Problem 6
\subsection{}

\end{document}
